src/StepDet.v
@@ -3,12 +3,24 @@ Require Import Common FMap Syntax Semantics.
 
 Inductive step_det (sys: System) : TState -> TLabel -> TState -> Prop :=
 | SdSlt: forall st, step_det sys st emptyILabel st
-| SdInt: forall ts oss oims obj oidx os pos (fmsg: TMsg) fpmsg fidx fchn outs,
+| SdExt: forall ts oss oims emsg,
+    isExternal sys (mid_from (msg_id emsg)) = true ->
+    isInternal sys (mid_to (msg_id emsg)) = true ->
+    step_det sys
+             {| tst_oss := oss; tst_msgs := oims; tst_tid := ts |}
+             (IlblIn (toTMsgU emsg))
+             {| tst_oss := oss;
+                tst_msgs := distributeMsg (toTMsgU emsg) oims;
+                tst_tid := ts
+             |}
+| SdIntFwd: forall ts mts oss oims obj oidx os pos
+                   (fmsg: TMsg) fpmsg fidx fchn outs,
     In obj (sys_objs sys) ->
     oidx = obj_idx obj ->
     (oss)@[oidx] = Some os ->
 
     isInternal sys (mid_from (msg_id (getMsg fmsg))) = true ->
+    tmsg_tid fmsg = Some mts ->
 
     ValidMsgId fidx oidx fchn fmsg ->
     firstM fidx oidx fchn oims = Some fmsg -> 
@@ -22,31 +34,35 @@ Inductive step_det (sys: System) : TState -> TLabel -> TState -> Prop :=
 
     step_det sys
              {| tst_oss := oss; tst_msgs := oims; tst_tid := ts |}
-             (IlblInt (Some fmsg) (extOuts sys (toTMsgs (tmsg_tid fmsg) outs)))
+             (IlblOuts (Some fmsg) (extOuts sys (toTMsgs mts outs)))
              {| tst_oss := oss +[ oidx <- pos ];
-                tst_msgs := distributeMsgs (intOuts sys (toTMsgs (tmsg_tid fmsg) outs)) oims;
+                tst_msgs := distributeMsgs (intOuts sys (toTMsgs mts outs)) oims;
                 tst_tid := ts
              |}
-
-| SdExt: forall ts nts (Hts: nts > ts) oss oims obj oidx os pos (emsg: Msg) fpmsg outs,
+| SdIntInit: forall ts nts (Hts: nts > ts) oss oims obj oidx os pos
+                   (fmsg: TMsg) fpmsg fidx fchn outs,
     In obj (sys_objs sys) ->
     oidx = obj_idx obj ->
-    oss@[oidx] = Some os ->
+    (oss)@[oidx] = Some os ->
 
-    isExternal sys (mid_from (msg_id emsg)) = true ->
+    isInternal sys (mid_from (msg_id (getMsg fmsg))) = true ->
+    tmsg_tid fmsg = None ->
 
-    msg_id emsg = pmsg_mid fpmsg ->
+    ValidMsgId fidx oidx fchn fmsg ->
+    firstM fidx oidx fchn oims = Some fmsg -> 
+
+    msg_id (getMsg fmsg) = pmsg_mid fpmsg ->
     In fpmsg (obj_trs obj) ->
     pmsg_precond fpmsg os ->
-    pmsg_postcond fpmsg os (msg_value emsg) pos ->
-    outs = pmsg_outs fpmsg os (msg_value emsg) ->
+    pmsg_postcond fpmsg os (msg_value (getMsg fmsg)) pos ->
+    outs = pmsg_outs fpmsg os (msg_value (getMsg fmsg)) ->
     ValidOuts oidx outs ->
 
     step_det sys
              {| tst_oss := oss; tst_msgs := oims; tst_tid := ts |}
-             (IlblExt {| tmsg_msg := emsg; tmsg_tid := nts |} (extOuts sys (toTMsgs nts outs)))
+             (IlblOuts (Some (toTMsg nts (getMsg fmsg))) (extOuts sys (toTMsgs nts outs)))
              {| tst_oss := oss +[ oidx <- pos ];
-                tst_msgs := distributeMsgs (intOuts sys (toTMsgs ts outs)) oims;
+                tst_msgs := distributeMsgs (intOuts sys (toTMsgs nts outs)) oims;
                 tst_tid := nts
              |}.
 
