src/StepSeq.v
@@ -1,56 +1,73 @@
 Require Import Bool List String Peano_dec.
 Require Import Permutation.
-Require Import Common FMap Syntax Semantics StepDet Serial.
+Require Import Common FMap Syntax Semantics StepDet.
 
 Inductive step_seq (sys: System) : TState -> TLabel -> TState -> Prop :=
 | SsSlt: forall st, step_seq sys st emptyILabel st
-| SsInt: forall ts oss oims obj idx os pos (fmsg: TMsg) fpmsg fidx fchn outs,
+| SsExt: forall ts oss oims emsg,
+    isExternal sys (mid_from (msg_id emsg)) = true ->
+    isInternal sys (mid_to (msg_id emsg)) = true ->
+    step_seq sys
+             {| tst_oss := oss; tst_msgs := oims; tst_tid := ts |}
+             (IlblIn (toTMsgU emsg))
+             {| tst_oss := oss;
+                tst_msgs := distributeMsg (toTMsgU emsg) oims;
+                tst_tid := ts
+             |}
+| SsIntFwd: forall ts oss oims obj oidx os pos
+                   (fmsg: TMsg) fpmsg fidx fchn outs,
     In obj (sys_objs sys) ->
-    idx = obj_idx obj ->
-    oss@[idx] = Some os ->
+    oidx = obj_idx obj ->
+    (oss)@[oidx] = Some os ->
 
     isInternal sys (mid_from (msg_id (getMsg fmsg))) = true ->
 
-    firstM fidx idx fchn oims = Some fmsg -> 
+    (* This is the only difference from [step_det]: internal forwarding happens
+     * only for the current transaction.
+     *)
+    tmsg_tid fmsg = Some ts ->
+
+    ValidMsgId fidx oidx fchn fmsg ->
+    firstM fidx oidx fchn oims = Some fmsg ->
+
     msg_id (getMsg fmsg) = pmsg_mid fpmsg ->
-    ValidMsgId fidx idx fchn fmsg ->
     In fpmsg (obj_trs obj) ->
     pmsg_precond fpmsg os ->
     pmsg_postcond fpmsg os (msg_value (getMsg fmsg)) pos ->
     outs = pmsg_outs fpmsg os (msg_value (getMsg fmsg)) ->
-    ValidOuts (obj_idx obj) outs ->
-
-    (* For internal steps, below is the only additional condition from [step_det]. *)
-    tmsg_tid fmsg = ts ->
+    ValidOuts oidx outs ->
 
     step_seq sys
-             {| tst_oss := oss;
-                tst_msgs := oims;
-                tst_tid := ts |}
-             (IlblInt (Some fmsg) (extOuts sys (toTMsgs (tmsg_tid fmsg) outs)))
-             {| tst_oss := oss +[ idx <- pos ];
-                tst_msgs := distributeMsgs (intOuts sys (toTMsgs (tmsg_tid fmsg) outs)) oims;
-                tst_tid := ts |}
-
-| SsExt: forall ts nts (Hts: nts > ts) oss oims obj os pos (emsg: Msg) fpmsg outs,
+             {| tst_oss := oss; tst_msgs := oims; tst_tid := ts |}
+             (IlblOuts (Some fmsg) (extOuts sys (toTMsgs ts outs)))
+             {| tst_oss := oss +[ oidx <- pos ];
+                tst_msgs := distributeMsgs (intOuts sys (toTMsgs ts outs)) oims;
+                tst_tid := ts
+             |}
+| SsIntInit: forall ts nts (Hts: nts > ts) oss oims obj oidx os pos
+                   (fmsg: TMsg) fpmsg fidx fchn outs,
     In obj (sys_objs sys) ->
-    oss@[obj_idx obj] = Some os ->
+    oidx = obj_idx obj ->
+    (oss)@[oidx] = Some os ->
 
-    isExternal sys (mid_from (msg_id emsg)) = true ->
+    isInternal sys (mid_from (msg_id (getMsg fmsg))) = true ->
+    tmsg_tid fmsg = None ->
 
-    msg_id emsg = pmsg_mid fpmsg ->
+    ValidMsgId fidx oidx fchn fmsg ->
+    firstM fidx oidx fchn oims = Some fmsg -> 
+
+    msg_id (getMsg fmsg) = pmsg_mid fpmsg ->
     In fpmsg (obj_trs obj) ->
     pmsg_precond fpmsg os ->
-    pmsg_postcond fpmsg os (msg_value emsg) pos ->
-    outs = pmsg_outs fpmsg os (msg_value emsg) ->
-    ValidOuts (obj_idx obj) outs ->
+    pmsg_postcond fpmsg os (msg_value (getMsg fmsg)) pos ->
+    outs = pmsg_outs fpmsg os (msg_value (getMsg fmsg)) ->
+    ValidOuts oidx outs ->
 
     step_seq sys
-             {| tst_oss := oss;
-                tst_msgs := oims;
-                tst_tid := ts |}
-             (IlblExt {| tmsg_msg := emsg; tmsg_tid := nts |} (extOuts sys (toTMsgs nts outs)))
-             {| tst_oss := oss +[ obj_idx obj <- pos ];
-                tst_msgs := distributeMsgs (intOuts sys (toTMsgs ts outs)) oims;
-                tst_tid := nts |}.
+             {| tst_oss := oss; tst_msgs := oims; tst_tid := ts |}
+             (IlblOuts (Some (toTMsg nts (getMsg fmsg))) (extOuts sys (toTMsgs nts outs)))
+             {| tst_oss := oss +[ oidx <- pos ];
+                tst_msgs := distributeMsgs (intOuts sys (toTMsgs nts outs)) oims;
+                tst_tid := nts
+             |}.
 
